examples/mtac/Patterns.v
@@ -1,0 +1,255 @@
+Require Import ExtLib.Core.RelDec.
+Require Import ExtLib.Structures.Monads.
+Require Import ExtLib.Structures.Traversable.
+Require Import ExtLib.Structures.Traversable.
+Require Import ExtLib.Data.List.
+Require Import ExtLib.Data.Monads.ReaderMonad.
+Require Import ExtLib.Data.Vector.
+Require Import ExtLib.Tactics.Cases.
+Require Import ExtLib.Tactics.Consider.
+Require Import MirrorCore.Ext.Expr.
+
+Set Implicit Arguments.
+Set Strict Implicit.
+
+(** Patterns Matching via unification **)
+Inductive mpattern :=
+| PGet (i : nat) (t : typ)
+| PVar (v : nat)
+| PUVar (u : uvar)
+| PFunc (f : func) (ls : list typ)
+| PApp (l r : mpattern)
+| PAbs (t : typ) (e : mpattern)
+| PEqual (t : typ) (l r : mpattern)
+| PNot (e : mpattern).
+
+(** The type of an [mpattern] **)
+Fixpoint typeof_mpattern (tfs : tfunctions) (tus tvs : list typ) (p : mpattern)
+: option typ :=
+  match p with
+    | PGet _ t => Some t
+    | PVar v => nth_error tvs v
+    | PUVar u => nth_error tus u
+    | PFunc f ts =>
+      match nth_error tfs f with
+        | Some r =>
+          if EqNat.beq_nat (length ts) (tfenv r)
+          then Some (instantiate_typ ts (tftype r))
+          else None
+        | None => None
+      end
+    | PApp l r =>
+      bind (typeof_mpattern tfs tus tvs l)
+           (fun tf =>
+              bind (typeof_mpattern tfs tus tvs r) (type_of_apply tf))
+    | PAbs t e =>
+      bind (typeof_mpattern tfs tus (t :: tvs) e)
+           (fun t' => ret (tvArr t t'))
+    | PEqual t l r =>
+      bind (typeof_mpattern tfs tus tvs l)
+           (fun tl => bind (typeof_mpattern tfs tus tvs r)
+                           (fun tr => if andb (t ?[ eq ] tl) (t ?[ eq ] tr)
+                                      then Some tvProp else None))
+    | PNot e =>
+      bind (typeof_mpattern tfs tus tvs e)
+           (fun tl => if tl ?[ eq ] tvProp then Some tvProp else None)
+  end.
+
+Fixpoint typecheck_mpattern (tgs : list typ) (p : mpattern) : bool :=
+  match p with
+    | PGet g t => nth_error tgs g ?[ eq ] Some t
+    | PVar _ => true
+    | PUVar _ => true
+    | PFunc _ _ => true
+    | PApp l r => if typecheck_mpattern tgs l then
+                    typecheck_mpattern tgs r
+                  else false
+    | PAbs _ e => typecheck_mpattern tgs e
+    | PEqual _ l r => if typecheck_mpattern tgs l then
+                        typecheck_mpattern tgs r
+                      else false
+    | PNot e => typecheck_mpattern tgs e
+  end.
+
+(** Convert an [mpattern] to an [expr]. [PGet] turn into unification
+ ** variables indexed from [Ubase].
+ **)
+Definition expr_of_mpattern (Ubase : uvar) : mpattern -> expr :=
+  fix recur (p : mpattern) : expr :=
+    match p with
+      | PGet u _ => UVar (Ubase + u)
+      | PVar v => Var v
+      | PUVar v => UVar v
+      | PFunc f ts => Func f ts
+      | PApp l r => App (recur l) (recur r)
+      | PAbs t e => Abs t (recur e)
+      | PEqual t l r => Equal t (recur l) (recur r)
+      | PNot e => Not (recur e)
+    end.
+
+Fixpoint list_join T (x y : list (option T)) : list (option T) :=
+  match x , y with
+    | nil , _ => y
+    | _ , nil => x
+    | x :: xs , y :: ys =>
+      match x , y with
+        | _ , None => x
+        | _ , y => y
+      end :: list_join xs ys
+  end.
+
+Fixpoint satisfies {T} (c : list (option T)) (ls : list T) : Prop :=
+  match c with
+    | nil => True
+    | None :: cs => match ls with
+                      | nil => False
+                      | _ :: ls => satisfies cs ls
+                    end
+    | Some c :: cs => match ls with
+                        | nil => False
+                        | l :: ls => l = c /\ satisfies cs ls
+                      end
+  end.
+
+Require Import ExtLib.Tactics.Injection.
+
+(*
+Lemma satisfies_join : forall T a b c,
+  satisfies (list_join (T := T) a b) c ->
+  satisfies b c.
+Proof.
+  induction a; destruct b; destruct c; simpl; forward_unsafe; inv_all; subst; auto.
+  {  destruct H0; subst.
+     eapply IHa in H0.
+
+Proof.
+  induction a; destruct b; destruct c; destruct d; simpl;
+  forward_unsafe; inv_all; subst; intuition; subst; intuition.
+  { 
+*)
+
+Fixpoint list_set (n : nat) (t : typ) (ls : list (option typ))
+: list (option typ) :=
+  match n with
+    | 0 => Some t :: tl ls
+    | S n => match ls with
+               | nil => None :: list_set n t nil
+               | t' :: ts => t' :: list_set n t ts
+             end
+  end.
+
+Fixpoint getEnv' (p : mpattern) (ls : list (option typ)) : option (list (option typ)) :=
+  match p with
+    | PGet u t =>
+      match nth_error ls u with
+        | None
+        | Some None => Some (list_set u t ls)
+        | Some (Some t') =>
+          if t ?[ eq ] t' then Some ls else None
+      end
+    | PVar _ => Some ls
+    | PFunc _ _ => Some ls
+    | PApp l r =>
+      bind (getEnv' l ls) (getEnv' r)
+    | PAbs _ e => getEnv' e ls
+    | PUVar _ => Some ls
+    | PEqual _ l r =>
+      bind (getEnv' l ls) (getEnv' r)
+    | PNot e => getEnv' e ls
+  end.
+
+Lemma satisfies_both : forall T p1 p2 tgs,
+                         satisfies p1 tgs ->
+                         satisfies p2 tgs ->
+                         satisfies (list_join (T := T) p1 p2) tgs.
+Proof.
+  induction p1; simpl; intros; auto.
+  forward_unsafe; intuition; subst; simpl in *; intuition.
+Qed.
+
+Lemma satisfies_nth_error : forall i tgs t,
+  nth_error tgs i ?[ eq ] Some t = true <->
+  satisfies (list_set i t nil) tgs.
+Proof.
+  induction i; destruct tgs; simpl; intros.
+  { intuition. }
+  { intuition.
+    consider (typ_eqb t t0); intuition.
+    subst. consider (typ_eqb t0 t0); intuition. }
+  { intuition. }
+  { eapply IHi. }
+Qed.
+
+Theorem getEnv_satisfies : forall a b c d,
+  satisfies c d ->
+  getEnv' a b = Some c ->
+  satisfies b d.
+Proof.
+  induction a; simpl; intros; forward_unsafe; subst; inv_all; subst; eauto.
+  { generalize dependent i. revert d.
+    induction b; simpl; intros; auto.
+    destruct i; simpl in *; forward; intuition; subst.
+    { inversion H2. }
+    { destruct a; intuition; subst; eauto. } }
+  { generalize dependent i. revert d.
+    induction b; simpl; intros; auto.
+    destruct i; simpl in *; forward; intuition; subst.
+    { inversion H2. }
+    { destruct a; intuition; subst; eauto. } }
+Qed.
+
+Theorem WellTyped_expr_expr_of_mpattern : forall tfs tus ptrn tvs tgs t,
+  typeof_mpattern tfs tus tvs ptrn = Some t ->
+  forall x tgs',
+    getEnv' ptrn x = Some tgs' ->
+    satisfies tgs' tgs ->
+    WellTyped_expr tfs (tus ++ tgs) tvs (expr_of_mpattern (length tus) ptrn) t.
+Proof.
+  unfold WellTyped_expr.
+  induction ptrn; simpl; intros; inv_all; subst; forward; eauto.
+  { rewrite ListNth.nth_error_app_R by omega.
+    replace (length tus + i - length tus) with i by omega.
+    forward_unsafe; subst.
+    { inv_all; subst.
+      generalize dependent tgs'. clear. revert tgs.
+      induction i; destruct tgs'; intuition; simpl in *;
+        unfold error, value in *; intuition; inv_all; subst; try congruence.
+      forward. destruct o; destruct tgs; intuition; subst; eauto. }
+    { inv_all.
+      rewrite <- rel_dec_correct.
+      clear - H2 H1. subst.
+      generalize dependent x; revert tgs.
+      induction i; destruct tgs; simpl; intros; intuition; subst.
+      consider (typ_eqb t0 t0); intuition.
+      destruct x; simpl in *; intuition try congruence.
+      destruct o; intuition.
+      destruct x; simpl in *; intuition try congruence; eauto.
+      destruct o; intuition eauto. }
+    { inv_all; subst.
+      clear - H1.
+      generalize dependent x. revert tgs.
+      induction i; simpl; intros; forward; intuition; subst; auto.
+      { destruct x; destruct tgs; simpl in *; intuition eauto.
+        destruct o; intuition.
+        destruct o; intuition eauto. } } }
+  { erewrite ListNth.nth_error_weaken; eauto. }
+  { erewrite IHptrn1; eauto.
+    erewrite IHptrn2; eauto.
+    eauto using getEnv_satisfies. }
+  { inv_all; subst.
+    erewrite IHptrn; eauto. }
+  { intuition; inv_all; subst. subst.
+    erewrite IHptrn1; eauto.
+    erewrite IHptrn2; eauto.
+    rewrite rel_dec_eq_true; eauto with typeclass_instances.
+    eauto using getEnv_satisfies. }
+  { inv_all; subst.
+    erewrite IHptrn; eauto.
+    rewrite rel_dec_eq_true; eauto with typeclass_instances. }
+Qed.
+
+Definition binders_of_mpattern (ptrn : mpattern) : option (list typ) :=
+  match getEnv' ptrn nil with
+    | None => None
+    | Some r => mapT (fun x => x) r
+  end.
